riscV/Asm.v
@@ -1399,103 +1399,105 @@ Inductive step: state -> trace -> state -> Prop :=
       forall (REC_CURCOMP: Genv.find_comp_ignore_offset ge (rs PC) = callee_comp st),
       step (State st rs m) t (ReturnState st rs' m').
 
-(* Two fixes: check sig when call CALLSIG, public & first order args when undefined external call LL *)
+(* Two fixes: check sig when call CALLSIG, public & first order args when undefined external call VISFO *)
 Inductive step_fix: state -> trace -> state -> Prop :=
-  | exec_step_fix_internal:
-      forall b ofs f i rs m rs' m' b' ofs' st cp,
-      rs PC = Vptr b ofs ->
-      Genv.find_funct_ptr ge b = Some (Internal f) ->
-      find_instr (Ptrofs.unsigned ofs) (fn_code f) = Some i ->
-      forall (COMP: comp_of f = cp),
+| exec_step_fix_internal:
+  forall b ofs f i rs m rs' m' b' ofs' st cp,
+    rs PC = Vptr b ofs ->
+    Genv.find_funct_ptr ge b = Some (Internal f) ->
+    find_instr (Ptrofs.unsigned ofs) (fn_code f) = Some i ->
+    forall (COMP: comp_of f = cp),
       exec_instr f i rs m cp = Next rs' m' ->
       sig_call i = None ->
       is_return i = false ->
       forall (NEXTPC: rs' PC = Vptr b' ofs'),
       forall (ALLOWED: cp = Genv.find_comp_ignore_offset ge (Vptr b' ofs')),
-      step_fix (State st rs m) E0 (State st rs' m')
-  | exec_step_fix_internal_call:
-      forall b ofs f i sig rs m rs' m' b' ofs' cp st st' args t,
-      rs PC = Vptr b ofs ->
-      Genv.find_funct_ptr ge b = Some (Internal f) ->
-      find_instr (Ptrofs.unsigned ofs) (fn_code f) = Some i ->
-      exec_instr f i rs m cp = Next rs' m' ->
-      sig_call i = Some sig ->
-      forall (NEXTPC: rs' PC = Vptr b' ofs'),
-      forall (ALLOWED: Genv.allowed_call ge (comp_of f) (Vptr b' ofs')),
-      forall (CURCOMP: Genv.find_comp_ignore_offset ge (Vptr b Ptrofs.zero) = cp),
-      (* Is a call, we update the stack *)
-      forall (STUPD: update_stack_call st sig cp rs' = Some st'),
-      forall (ARGS: call_arguments rs' m' sig args),
-      (* Is a call, we check whether we are allowed to pass pointers *)
-      forall (NO_CROSS_PTR:
-          Genv.type_of_call ge (comp_of f) (Genv.find_comp_ignore_offset ge (Vptr b' ofs')) = Genv.CrossCompartmentCall ->
-          List.Forall not_ptr args),
-      forall (EV: call_trace ge (comp_of f) (Genv.find_comp_ignore_offset ge (Vptr b' ofs')) (Vptr b' ofs') args (sig_args sig) t),
-      (* Check signature *)
-      forall (CALLSIG: Genv.type_of_call ge (comp_of f) (Genv.find_comp_ignore_offset ge (Vptr b' ofs')) <> Genv.InternalCall ->
-                    (exists fd, Genv.find_funct_ptr ge b' = Some fd /\ sig = funsig fd)),
+        step_fix (State st rs m) E0 (State st rs' m')
+| exec_step_fix_internal_call:
+  forall b ofs f i sig rs m rs' m' b' ofs' cp st st' args t,
+    rs PC = Vptr b ofs ->
+    Genv.find_funct_ptr ge b = Some (Internal f) ->
+    find_instr (Ptrofs.unsigned ofs) (fn_code f) = Some i ->
+    exec_instr f i rs m cp = Next rs' m' ->
+    sig_call i = Some sig ->
+    forall (NEXTPC: rs' PC = Vptr b' ofs'),
+    forall (ALLOWED: Genv.allowed_call ge (comp_of f) (Vptr b' Ptrofs.zero)),
+    forall (CURCOMP: Genv.find_comp_ignore_offset ge (Vptr b Ptrofs.zero) = cp),
+    (* Is a call, we update the stack *)
+    forall (STUPD: update_stack_call st sig cp rs' = Some st'),
+    forall (ARGS: call_arguments rs' m' sig args),
+    (* Is a call, we check whether we are allowed to pass pointers *)
+    forall (NO_CROSS_PTR:
+        Genv.type_of_call ge (comp_of f) (Genv.find_comp_ignore_offset ge (Vptr b' ofs')) = Genv.CrossCompartmentCall ->
+        List.Forall not_ptr args),
+    forall (EV: call_trace ge (comp_of f) (Genv.find_comp_ignore_offset ge (Vptr b' ofs')) (Vptr b' ofs')
+                      args (sig_args sig) t),
+    (* Check signature *)
+    forall (CALLSIG: Genv.type_of_call ge (comp_of f) (Genv.find_comp_ignore_offset ge (Vptr b' ofs')) <> Genv.InternalCall ->
+                (exists fd, Genv.find_funct_ptr ge b' = Some fd /\ sig = funsig fd)),
       step_fix (State st rs m) t (State st' rs' m')
-  | exec_step_fix_internal_return:
-      forall b ofs f i rs m rs' cp m' st,
-      rs PC = Vptr b ofs ->
-      Genv.find_funct_ptr ge b = Some (Internal f) ->
-      find_instr (Ptrofs.unsigned ofs) (fn_code f) = Some i ->
-      exec_instr f i rs m cp = Next rs' m' ->
-      is_return i = true ->
-      forall (CURCOMP: Genv.find_comp_ignore_offset ge (rs PC) = cp),
-      (* We attempt a return, so we go to a ReturnState*)
-      (* The only condition is the following: we are currently in the compartment stored in the callee compartment field
+| exec_step_fix_internal_return:
+  forall b ofs f i rs m rs' cp m' st,
+    rs PC = Vptr b ofs ->
+    Genv.find_funct_ptr ge b = Some (Internal f) ->
+    find_instr (Ptrofs.unsigned ofs) (fn_code f) = Some i ->
+    exec_instr f i rs m cp = Next rs' m' ->
+    is_return i = true ->
+    forall (CURCOMP: Genv.find_comp_ignore_offset ge (rs PC) = cp),
+    (* We attempt a return, so we go to a ReturnState*)
+    (* The only condition is the following: we are currently in the compartment stored in the callee compartment field
        of the top stack frame*)
-      forall (REC_CURCOMP: Genv.find_comp_ignore_offset ge (rs PC) = callee_comp st),
+    forall (REC_CURCOMP: Genv.find_comp_ignore_offset ge (rs PC) = callee_comp st),
       (* forall (NEXTCOMP: Genv.find_comp_ignore_offset ge (rs' PC) = cp'), *)
       step_fix (State st rs m) E0 (ReturnState st rs' m')
-  | exec_step_fix_return:
-      forall st st' rs m sg t rec_cp rec_cp' cp',
-        rs PC <> Vnullptr -> (* this condition is there to stop the execution 1 step_fix earlier, to make the proof easier *)
-        forall (REC_CURCOMP: callee_comp st = rec_cp),
-        forall (REC_NEXTCOMP: call_comp st = rec_cp'),
-        forall (NEXTCOMP: Genv.find_comp_ignore_offset ge (rs PC) = cp'),
-        (* We only impose conditions on when returns can be executed for cross-compartment
+| exec_step_fix_return:
+  forall st st' rs m sg t rec_cp rec_cp' cp',
+    rs PC <> Vnullptr -> (* this condition is there to stop the execution 1 step_fix earlier, to make the proof easier *)
+    forall (REC_CURCOMP: callee_comp st = rec_cp),
+    forall (REC_NEXTCOMP: call_comp st = rec_cp'),
+    forall (NEXTCOMP: Genv.find_comp_ignore_offset ge (rs PC) = cp'),
+    (* We only impose conditions on when returns can be executed for cross-compartment
            returns. These conditions are that we restore the previous RA and SP *)
-        forall (PC_RA: rec_cp <> cp' -> rs PC = asm_parent_ra st),
-        forall (RESTORE_SP: rec_cp <> cp' -> rs SP = asm_parent_sp st),
-        (* forall (RETURN_FROM_CP: cp <> cp' -> cp = callee_comp st), *)
-        (* Note that in the same manner, this definition only updates the stack when doing
+    forall (PC_RA: rec_cp <> cp' -> rs PC = asm_parent_ra st),
+    forall (RESTORE_SP: rec_cp <> cp' -> rs SP = asm_parent_sp st),
+    (* forall (RETURN_FROM_CP: cp <> cp' -> cp = callee_comp st), *)
+    (* Note that in the same manner, this definition only updates the stack when doing
          cross-compartment returns *)
-        forall (STUPD: update_stack_return st rec_cp rs = Some st'),
-        (* We do not return a pointer *)
-        forall (SIG_STACK: sig_of_call st = sg),
-        forall (NO_CROSS_PTR:
-            (Genv.type_of_call ge cp' rec_cp = Genv.CrossCompartmentCall ->
-             not_ptr (return_value rs sg))),
-        forall (EV: return_trace ge cp' rec_cp (return_value rs sg) (sig_res sg) t),
-          step_fix (ReturnState st rs m) t (State st' rs m)
-  | exec_step_fix_builtin:
-      forall b ofs f ef args res rs m vargs t vres rs' m' st,
-      rs PC = Vptr b ofs ->
-      Genv.find_funct_ptr ge b = Some (Internal f) ->
-      find_instr (Ptrofs.unsigned ofs) f.(fn_code) = Some (Pbuiltin ef args res) ->
-      eval_builtin_args ge rs (rs SP) m args vargs ->
-      external_call ef ge (comp_of f) vargs m t vres m' ->
+    forall (STUPD: update_stack_return st rec_cp rs = Some st'),
+    (* We do not return a pointer *)
+    forall (SIG_STACK: sig_of_call st = sg),
+    forall (NO_CROSS_PTR:
+        (Genv.type_of_call ge cp' rec_cp = Genv.CrossCompartmentCall ->
+         not_ptr (return_value rs sg))),
+    forall (EV: return_trace ge cp' rec_cp (return_value rs sg) (sig_res sg) t),
+      step_fix (ReturnState st rs m) t (State st' rs m)
+| exec_step_fix_builtin:
+  forall b ofs f ef args res rs m vargs t vres rs' m' st,
+    rs PC = Vptr b ofs ->
+    Genv.find_funct_ptr ge b = Some (Internal f) ->
+    find_instr (Ptrofs.unsigned ofs) f.(fn_code) = Some (Pbuiltin ef args res) ->
+    eval_builtin_args ge rs (rs SP) m args vargs ->
+    external_call ef ge vargs m t vres m' ->
+    forall (ALLOWED: comp_of ef = comp_of f),
       rs' = nextinstr
               (set_res res vres
-                (undef_regs (map preg_of (destroyed_by_builtin ef))
-                   (rs #X1 <- Vundef #X31 <- Vundef))) ->
+                       (undef_regs (map preg_of (destroyed_by_builtin ef))
+                                   (rs #X1 <- Vundef #X31 <- Vundef))) ->
       (* Limit leaks when calling unknown function *)
-      forall (LL: limit_leaks_if_unknown ef ge m vargs),
-      step_fix (State st rs m) t (State st rs' m')
-  | exec_step_fix_external:
-      forall b ef args res rs m t rs' m' cp st,
-      rs PC = Vptr b Ptrofs.zero ->
-      Genv.find_funct_ptr ge b = Some (External ef) ->
-      forall COMP: Genv.find_comp_ignore_offset ge (rs RA) = cp, (* compartment that is calling the external function *)
-      external_call ef ge cp args m t res m' ->
-      extcall_arguments rs m (ef_sig ef) args ->
-      rs' = (set_pair (loc_external_result (ef_sig ef)) res (undef_caller_save_regs rs))#PC <- (rs RA) ->
-      (* These step_fixs behave like returns. So we do the same as in the [exec_step_fix_internal_return] case. *)
-      forall (REC_CURCOMP: Genv.find_comp_ignore_offset ge (rs PC) = callee_comp st),
-      (* Limit leaks when calling unknown function *)
-      forall (LL: limit_leaks_if_unknown ef ge m args),
+      forall (VISFO: visible_fo_if_unknown ef ge m vargs),
+        step_fix (State st rs m) t (State st rs' m')
+| exec_step_fix_external:
+  forall b ef args res rs m t rs' m' st,
+    rs PC = Vptr b Ptrofs.zero ->
+    Genv.find_funct_ptr ge b = Some (External ef) ->
+    (* forall COMP: Genv.find_comp_ignore_offset ge (rs RA) = cp, (* compartment that is calling the external function *) *)
+    external_call ef ge args m t res m' ->
+    extcall_arguments rs m (ef_sig ef) args ->
+    rs' = (set_pair (loc_external_result (ef_sig ef)) res (undef_caller_save_regs rs))#PC <- (rs RA) ->
+    (* These steps behave like returns. So we do the same as in the [exec_step_internal_return] case. *)
+    forall (REC_CURCOMP: Genv.find_comp_ignore_offset ge (rs PC) = callee_comp st),
+    (* Limit leaks when calling unknown function *)
+    forall (VISFO: visible_fo_if_unknown ef ge m args),
       step_fix (State st rs m) t (ReturnState st rs' m').
 
 End RELSEM.
